Worked on Values.v

src/Language/PlutusIR/Semantics/Dynamic/Values.v
@@ -1,30 +1,60 @@
 Require Import PlutusCert.Language.PlutusIR.
+Require Import PlutusCert.Util.
 Import NamedTerm.
 Require Import PlutusCert.Language.PlutusIR.Semantics.Dynamic.BuiltinMeanings.
 From Coq Require Import Bool.Bool Arith.PeanoNat.
-Import PeanoNat.Nat.
+
+From QuickChick Require Import QuickChick.
+
 
 Inductive is_error : Term -> Prop :=
   | IsError : forall T,
       is_error (Error T).
 
-Inductive value : Term -> Prop :=
-  | V_LamAbs : forall x T t0,
-      value (LamAbs x T t0) 
-  | V_TyAbs : forall X K t,
-      value (TyAbs X K t)
-  | V_IWrap : forall F T v,
-      value v ->
+QCDerive DecOpt for (is_error tm).
+
+Instance is_error_DecOpt_sound tm : DecOptSoundPos (is_error tm).
+Proof. derive_sound. Qed.
+
+Instance is_error_ty_DecOpt_complete tm : DecOptCompletePos (is_error tm).
+Proof. derive_complete. Qed.
+
+Instance is_error_ty_DecOpt_monotonic tm : DecOptSizeMonotonic (is_error tm).
+Proof. derive_mon. Qed.
+
+
+
+
+Inductive neutral_flag :=
+  | NFT
+  | NFF.
+
+Inductive value' : neutral_flag -> nat -> Term -> Prop :=
+  | V_LamAbs : forall n x T t0,
+      value' NFF n (LamAbs x T t0) 
+  | V_TyAbs : forall n X K t,
+      value' NFF n (TyAbs X K t)
+  | V_IWrap : forall n F T v,
+      value' NFF n v ->
       ~ is_error v ->
-      value (IWrap F T v)
-  | V_Constant : forall u,
-      value (Constant u)
-  | V_Error : forall T,
-      value (Error T)
+      value' NFF n (IWrap F T v)
+  | V_Constant : forall n u,
+      value' NFF n (Constant u)
+  | V_Error : forall n T,
+      value' NFF n (Error T)
   (** Builtins *) 
-  | V_Neutral : forall nv,
-      neutral_value 0 nv ->
-      value nv
+  | V_Neutral_Builtin : forall nf n f,
+      (* lt_nat (S n) (arity f) -> *)
+      value' nf n (Builtin f)
+  | V_Neutral_Apply : forall nf n nv v,
+      value' NFF 0 v ->
+      ~ is_error v ->
+      value' NFT (S n) nv ->
+      value' nf n (Apply nv v)
+  | V_Neutral_TyInst : forall nf n nv T,
+      value' NFT (S n) nv ->
+      value' nf n (TyInst nv T).
+
   (** If-Then-Else constructs 
 
       NOTE (2021-11-4): Removed separate treatment of if-then-else for the sake of simplicity.
@@ -38,35 +68,35 @@ Inductive value : Term -> Prop :=
   | V_If3 : forall T cond t,
       value (Apply (Apply (TyInst (Builtin IfThenElse) T) cond) t) *)
 
-with neutral_value : nat -> Term -> Prop :=
-  | NV_Builtin : forall n f,
-      (* NOTE (2021-11-4): Removed separate treatment of if-then-else for the sake of simplicity. *)
-      (* f <> IfThenElse -> *)
-      n < arity f ->
-      neutral_value n (Builtin f)
-  | NV_Apply : forall n nv v,
-      value v ->
-      ~ is_error v ->
-      neutral_value (S n) nv ->
-      neutral_value n (Apply nv v)
-  | NV_TyInst : forall n nv T,
-      neutral_value (S n) nv ->
-      neutral_value n (TyInst nv T)
-  .
+#[export] Hint Constructors value' : core.
 
-#[export] Hint Constructors value : core.
-#[export] Hint Constructors neutral_value : core.
-
-Scheme value__ind := Minimality for value Sort Prop
-  with neutral_value__ind := Minimality for neutral_value Sort Prop.
+Scheme value__ind := Minimality for value' Sort Prop.
 
 Combined Scheme value__multind from 
-  value__ind,
-  neutral_value__ind.
+  value__ind.
 
+Definition value (tm : Term) := value' NFF 0 tm.
+Definition neutral_value (n : nat) (t : Term) := value' NFT n t.
 Definition neutral (t : Term) := neutral_value 0 t.
 
 #[export] Hint Unfold neutral : core.
+#[export] Hint Unfold value : core.
+
+
+QCDerive DecOpt for (value' nt n tm).
+
+Instance value'_DecOpt_sound nt n tm : DecOptSoundPos (value' nt n tm).
+Proof. derive_sound. Qed.
+
+(* Some extra work is necessary to get around the value alias, QuickChick cannot do this itself *)
+Instance DecOptvalue tm : DecOpt (value tm) :=
+  {| decOpt s := @decOpt (value' NFF 0 tm) _ s |}.
+
+Instance value_DecOpt_sound tm : DecOptSoundPos (value tm).
+Proof. unfold value. unfold DecOptSoundPos. intros. apply sound with (s0 := s). apply H. Qed.
+
+
+
 
 Inductive fully_applied_neutral : nat -> Term -> Prop :=
   | FA_Builtin : forall n f,
@@ -97,15 +127,16 @@ Lemma neutral_value__monotone : forall n m nv,
     m <= n ->
     neutral_value m nv.
 Proof with (eauto || (try lia)).
+  unfold neutral_value.
   intros.
   generalize dependent m.
   induction H; intros...
-  - destruct f...
-    all: econstructor...
+  - constructor; try assumption.
+    apply IHvalue'2.
+    apply le_n_S.
+    apply H2.
   - econstructor...
-    eapply IHneutral_value...
-  - econstructor...
-    eapply IHneutral_value...
+    eapply IHvalue'...
 Qed.
 
 Lemma fully_applied_neutral__subsumes__neutral_value : forall m n nv,
@@ -113,10 +144,10 @@ Lemma fully_applied_neutral__subsumes__neutral_value : forall m n nv,
   m < n ->
   neutral_value m nv.
 Proof with (eauto || (try lia)).
+  unfold neutral_value.
   intros.
   generalize dependent m.
   induction H; intros...
-  - subst...
   - econstructor...
     eapply IHfully_applied_neutral...
   - econstructor...
@@ -148,7 +179,7 @@ Fixpoint
 
 
     (* Duplication for the termination checker *)
-    | Builtin f   => ltb n (arity f)
+    | Builtin f   => Nat.ltb n (arity f)
     | Apply nv v  => is_value' n v && negb (is_error_b v) && is_value' (S n) nv
     | TyInst nv T => is_value' (S n) nv
     | _ => false
